hax-lib/proof-libs/fstar/core/Core_models.Iter.Traits.Collect.fst
@@ -10,3 +10,12 @@ class t_IntoIterator (v_Self: Type0) = {
   f_into_iter:x0: v_Self
     -> Prims.Pure f_IntoIter (f_into_iter_pre x0) (fun result -> f_into_iter_post x0 result)
 }
+
+class t_FromIterator (v_Self: Type0) (v_A: Type0) = {
+  f_from_iter_pre:#v_T: Type0 -> {| i1: t_IntoIterator v_T |} -> v_T -> Type0;
+  f_from_iter_post:#v_T: Type0 -> {| i1: t_IntoIterator v_T |} -> v_T -> v_Self -> Type0;
+  f_from_iter:#v_T: Type0 -> {| i1: t_IntoIterator v_T |} -> x0: v_T
+    -> Prims.Pure v_Self
+        (f_from_iter_pre #v_T #i1 x0)
+        (fun result -> f_from_iter_post #v_T #i1 x0 result)
+}
