hax-lib/proof-libs/fstar/core/Alloc.Slice.fst
@@ -9,9 +9,8 @@ let impl__to_vec (#v_T: Type0) (s: t_Slice v_T) : Alloc.Vec.t_Vec v_T Alloc.Allo
   <:
   Alloc.Vec.t_Vec v_T Alloc.Alloc.t_Global
 
-let impl__into_vec (#v_T #v_A: Type0) (s: Alloc.Boxed.t_Box (t_Slice v_T) v_A)
-    : Alloc.Vec.t_Vec v_T v_A =
-  Alloc.Vec.Vec (Rust_primitives.Sequence.seq_from_slice #v_T s.Alloc.Boxed._0)
+let impl__into_vec (#v_T #v_A: Type0) (s: t_Slice v_T) : Alloc.Vec.t_Vec v_T v_A =
+  Alloc.Vec.Vec (Rust_primitives.Sequence.seq_from_slice #v_T s)
     (Core_models.Marker.PhantomData <: Core_models.Marker.t_PhantomData v_A)
   <:
   Alloc.Vec.t_Vec v_T v_A
