hax-lib/proof-libs/fstar/core/Std.Io.Impls.fsti
@@ -5,3 +5,6 @@ open Rust_primitives
 
 [@@ FStar.Tactics.Typeclasses.tcinstance]
 val impl:Std.Io.t_Read (t_Slice u8)
+
+[@@ FStar.Tactics.Typeclasses.tcinstance]
+val impl_1:Std.Io.t_Write (Alloc.Vec.t_Vec u8 Alloc.Alloc.t_Global)
